code/experimental/rsa/Hacl.Impl.Multiplication.fst
@@ -35,16 +35,15 @@ let rec bn_mult_by_limb_addj #aLen aaLen a l i j resLen carry res =
     let ij = add #SIZE i j in
     if (i <. aaLen) then begin
         let res_ij = res.(ij) in
-	let (carry', res_ij) = bn_mul_by_limb_addj_f a.(i) l carry res_ij in
+        let (carry', res_ij) = bn_mul_by_limb_addj_f a.(i) l carry res_ij in
         res.(ij) <- res_ij;
         bn_mult_by_limb_addj aaLen a l (size_incr i) j resLen carry' res end
-    else
-        res.(ij) <- carry
+    else res.(ij) <- carry
 
 val bn_mult_:
     #aLen:size_nat -> #bLen:size_nat ->
     aaLen:size_t{v aaLen == aLen} -> a:lbignum aLen ->
-    bbLen:size_t{v bbLen == bLen /\ aLen + bLen < max_size_t} -> b:lbignum bLen ->
+    bbLen:size_t{v bbLen == bLen} -> b:lbignum bLen ->
     j:size_t{v j <= bLen} ->
     resLen:size_t{v resLen = aLen + bLen} -> res:lbignum (aLen + bLen) -> Stack unit
     (requires (fun h -> live h a /\ live h b /\ live h res /\ disjoint res a /\ disjoint res b))
@@ -63,7 +62,7 @@ val bn_mul:
     bbLen:size_t{v bbLen == bLen /\ aLen + bLen < max_size_t} -> b:lbignum bLen ->
     res:lbignum (aLen + bLen) -> Stack unit
     (requires (fun h -> live h a /\ live h b /\ live h res /\ disjoint res a /\ disjoint res b))
-    (ensures (fun h0 _ h1 -> preserves_live h0 h1 /\ modifies1 res h0 h1))    
+    (ensures (fun h0 _ h1 -> preserves_live h0 h1 /\ modifies1 res h0 h1))
     [@"c_inline"]
 let bn_mul #aLen #bLen aaLen a bbLen b res =
     let resLen = add #SIZE aaLen bbLen in
@@ -101,7 +100,7 @@ let rec bn_sqr_sqr #aLen aaLen a i res =
     end
 
 val bn_sqr_:
-    #aLen:size_nat ->
+    #aLen:size_nat{aLen > 0} ->
     aaLen:size_t{v aaLen == aLen /\ aLen + aLen < max_size_t} -> a:lbignum aLen ->
     i:size_t{v i <= aLen} ->
     resLen:size_t{v resLen == aLen + aLen} -> res:lbignum (aLen + aLen) -> Stack unit
@@ -115,11 +114,12 @@ let rec bn_sqr_ #aLen aaLen a i resLen res =
     end
 
 val bn_sqr:
-    #aLen:size_nat ->
+    #aLen:size_nat{aLen > 0} ->
     aaLen:size_t{v aaLen == aLen /\ aLen + aLen < max_size_t} -> a:lbignum aLen ->
     tmp:lbignum (aLen + aLen) -> res:lbignum (aLen + aLen) -> Stack unit
-    (requires (fun h -> live h a /\ live h res /\ disjoint res a))
-    (ensures (fun h0 _ h1 -> preserves_live h0 h1 /\ modifies1 res h0 h1))
+    (requires (fun h -> live h a /\ live h res /\ live h tmp /\ 
+                      disjoint res a /\ disjoint tmp a /\ disjoint res tmp))
+    (ensures (fun h0 _ h1 -> preserves_live h0 h1 /\ modifies2 res tmp h0 h1))
     [@"c_inline"]
 let bn_sqr #aLen aaLen a tmp res =
     let resLen = add #SIZE aaLen aaLen in
@@ -129,32 +129,38 @@ let bn_sqr #aLen aaLen a tmp res =
     bn_sqr_sqr aaLen a (size 0) tmp;
     bn_add resLen res resLen tmp res
 
-val abs:
-    #aLen:size_nat -> #bLen:size_nat ->
-    aaLen:size_t{v aaLen == aLen} -> a:lbignum aLen ->
-    bbLen:size_t{v bbLen == bLen} -> b:lbignum aLen ->
-    res:lbignum aLen -> Stack unit
-    (requires (fun h -> live h a /\ live h b /\ live h res /\ disjoint a b))
-    (ensures  (fun h0 _ h1 -> preserves_live h0 h1 /\ modifies1 res h0 h1))
-    [@"c_inline"]
-let abs #aLen #bLen aaLen a bbLen b res =
-    if (bn_is_less aaLen a bbLen b) then
-       //a < b ==> res = b - a
-       bn_sub bbLen b aaLen a res
-    else bn_sub aaLen a bbLen b res
-
 type sign =
      | Positive : sign
      | Negative : sign
 
+val abs:
+    #aLen:size_nat -> #bLen:size_nat ->
+    aaLen:size_t{v aaLen == aLen} -> a:lbignum aLen ->
+    bbLen:size_t{v bbLen == bLen /\ bLen <= aLen} -> b:lbignum bLen ->
+    res:lbignum aLen -> Stack sign
+    (requires (fun h -> live h a /\ live h b /\ live h res /\ disjoint a b))
+    (ensures  (fun h0 _ h1 -> preserves_live h0 h1 /\ modifies1 res h0 h1))
+    [@"c_inline"]
+let abs #aLen #bLen aaLen a bbLen b res =
+    if (bn_is_less aaLen a bbLen b) //a < b
+    then begin
+      let a' = Buffer.sub #uint64 #aLen #bLen a (size 0) bbLen in
+      let res' = Buffer.sub #uint64 #aLen #bLen res (size 0) bbLen in
+      bn_sub bbLen b bbLen a' res';
+      Negative end
+    else begin
+      bn_sub aaLen a bbLen b res;
+      Positive end
+
 val add_sign:
     #a0Len:size_nat -> #a1Len:size_nat -> #resLen:size_nat ->
     aa0Len:size_t{v aa0Len == a0Len} ->
-    aa1Len:size_t{v aa1Len == a1Len} ->
+    aa1Len:size_t{v aa1Len == a1Len /\ a1Len <= a0Len} ->
     rresLen:size_t{v rresLen == resLen /\ resLen = a0Len + a0Len + 1 /\ resLen < max_size_t} ->
     c0:lbignum (a0Len + a0Len) -> c1:lbignum (a1Len + a1Len) -> c2:lbignum (a0Len + a0Len) ->
     a0:lbignum a0Len -> a1:lbignum a1Len -> a2:lbignum a0Len ->
     b0:lbignum a0Len -> b1:lbignum a1Len -> b2:lbignum a0Len ->
+    sa2:sign -> sb2:sign ->
     res:lbignum (v rresLen) -> Stack unit
     (requires (fun h -> live h c0 /\ live h c1 /\ live h c2 /\ 
                       live h a0 /\ live h a1 /\ live h a2 /\
@@ -162,110 +168,114 @@ val add_sign:
 		      live h res /\ disjoint a0 a1 /\ disjoint b0 b1))
     (ensures (fun h0 _ h1 -> preserves_live h0 h1 /\ modifies1 res h0 h1))
     [@"c_inline"]
-let add_sign #a0Len #a1Len #resLen aa0Len aa1Len rresLen c0 c1 c2 a0 a1 a2 b0 b1 b2 res =
+let add_sign #a0Len #a1Len #resLen aa0Len aa1Len rresLen c0 c1 c2 a0 a1 a2 b0 b1 b2 sa2 sb2 res =
     let c0Len = add #SIZE aa0Len aa0Len in
     let c1Len = add #SIZE aa1Len aa1Len in
-    let sa2 = if (bn_is_less aa0Len a0 aa1Len a1) then Negative else Positive in
-    let sb2 = if (bn_is_less aa0Len b0 aa1Len b1) then Negative else Positive in
     bn_add_carry c0Len c0 c1Len c1 res;
     if ((sa2 = Positive && sb2 = Positive) || (sa2 = Negative && sb2 = Negative))
     then bn_sub rresLen res c0Len c2 res
     else bn_add rresLen res c0Len c2 res
-    
+
+//modifies2 res tmp h0 h1
 val karatsuba_:
     #aLen:size_nat ->
-    pow2_i:size_t -> iLen:size_t ->
-    aaLen:size_t{v aaLen == aLen /\ 4 * v pow2_i < max_size_t /\ aLen + aLen < max_size_t} ->
+    pow2_i:size_t{4 * v pow2_i < max_size_t} -> iLen:size_t{v iLen < v pow2_i / 2} ->
+    aaLen:size_t{v aaLen == aLen /\ aLen + aLen < max_size_t /\ v iLen + aLen = v pow2_i} ->
     a:lbignum aLen -> b:lbignum aLen ->
     tmp:lbignum (4 * v pow2_i) ->
     res:lbignum (aLen + aLen) -> Stack unit
-    (requires (fun h -> live h a /\ live h b /\ live h tmp /\ live h res))
+    (requires (fun h -> live h a /\ live h b /\ live h tmp /\ live h res /\
+                      disjoint res a /\ disjoint res b /\ disjoint tmp a /\ disjoint tmp b))
     (ensures  (fun h0 _ h1 -> preserves_live h0 h1))
+    #reset-options "--z3rlimit 150 --max_fuel 2"
     [@"c_inline"]
 let rec karatsuba_ #aLen pow2_i iLen aaLen a b tmp res =
-    assume (v pow2_i = aLen + v iLen);
     let tmpLen = mul #SIZE (size 4) pow2_i in
-    let aaLen2 = add #SIZE aaLen aaLen in
+    let resLen = add #SIZE aaLen aaLen in
     let pow2_i0 = pow2_i /. (size 2) in
     assume (v pow2_i = v pow2_i0 + v pow2_i0);
-    let pow2_i1 = sub #SIZE pow2_i0 iLen in
     
     if (aaLen <. size 32) then
        bn_mul #aLen #aLen aaLen a aaLen b res
     else begin
        let a0 = Buffer.sub #uint64 #aLen #(v pow2_i0) a (size 0) pow2_i0 in
-       let a1 = Buffer.sub #uint64 #aLen #(v pow2_i1) a pow2_i0 pow2_i1 in
        let b0 = Buffer.sub #uint64 #aLen #(v pow2_i0) b (size 0) pow2_i0 in
-       let b1 = Buffer.sub #uint64 #aLen #(v pow2_i1) b pow2_i0 pow2_i1 in
 
        let tmp0 = Buffer.sub #uint64 #(v tmpLen) #(4 * v pow2_i0) tmp (size 0) (mul #SIZE (size 4) pow2_i0) in
-       let c0 = Buffer.sub #uint64 #(v aaLen2) #(2 * v pow2_i0) res (size 0) (mul #SIZE (size 2) pow2_i0) in
+       let c0 = Buffer.sub #uint64 #(v resLen) #(v pow2_i) res (size 0) pow2_i in
        karatsuba_ #(v pow2_i0) pow2_i0 (size 0) pow2_i0 a0 b0 tmp0 c0; // c0 = a0 * b0
 
+       let pow2_i1 = sub #SIZE pow2_i0 iLen in
        if (pow2_i1 =. size 1) then begin
+          let a1 = Buffer.sub #uint64 #aLen #1 a pow2_i0 (size 1) in
+          let b1 = Buffer.sub #uint64 #aLen #1 b pow2_i0 (size 1) in
           let a1_0 = a1.(size 0) in
           let b1_0 = b1.(size 0) in
+	  
           let c1 = mul_wide a1_0 b1_0 in
-          let c1_0 = to_u64 #U128 c1 in
-          let c1_1 = to_u64 #U128 (shift_right #U128 c1 (u32 64)) in
-          let c0Len = mul #SIZE (size 2) pow2_i0 in
-          res.(c0Len) <- c1_0;
-          res.(add #SIZE c0Len (size 1)) <- c1_1;
+          res.(pow2_i) <- to_u64 #U128 c1;
+          res.(size_incr pow2_i) <- to_u64 #U128 (shift_right #U128 c1 (u32 64));
 
-          let tmp0 = Buffer.sub #uint64 #(v tmpLen) #(v pow2_i0 + 1) tmp (size 0) (add #SIZE pow2_i0 (size 1)) in //tmp0 = a0 * b1_0
-          bn_mul_u64 #(v pow2_i0) pow2_i0 a0 b1_0 tmp0;
-          let tmp1 = Buffer.sub #uint64 #(v tmpLen) #(v pow2_i0 + 1) tmp (add #SIZE pow2_i0 (size 1)) (add #SIZE pow2_i0 (size 1)) in //tmp1 = b0 * a1_0
-          bn_mul_u64 #(v pow2_i0) pow2_i0 b0 a1_0 tmp1;
-          let tmp1Len = add #SIZE pow2_i0 (size 1) in
+          let tmp1Len = size_incr pow2_i0 in
           let tmp1Len2 = add #SIZE tmp1Len tmp1Len in
           let tmp2Len = add #SIZE pow2_i0 (size 2) in
-          let tmp2 = Buffer.sub #uint64 #(v tmpLen) #(v tmp2Len) tmp tmp1Len2 tmp2Len in //tmp2 = tmp0 + tmp1 = a0 * b1_0 + b0 * a1_0
-          bn_add_carry #(v tmp1Len) #(v tmp1Len) tmp1Len tmp0 tmp1Len tmp1 tmp2;
 	  
-          let res1Len = add #SIZE pow2_i0 (size 2) in
-          let res1 = Buffer.sub #uint64 #(v aaLen2) #(v res1Len) res pow2_i0 res1Len in
-          bn_add res1Len res1 tmp2Len tmp2 res1
+          let tmp0 = Buffer.sub #uint64 #(v tmpLen) #(v tmp1Len) tmp (size 0) tmp1Len in
+          let tmp1 = Buffer.sub #uint64 #(v tmpLen) #(v tmp1Len) tmp tmp1Len tmp1Len in
+          let tmp2 = Buffer.sub #uint64 #(v tmpLen) #(v tmp2Len) tmp tmp1Len2 tmp2Len in
+          let res1 = Buffer.sub #uint64 #(v resLen) #(v tmp2Len) res pow2_i0 tmp2Len in
+	  
+          bn_mul_u64 #(v pow2_i0) pow2_i0 a0 b1_0 tmp0; // tmp0 = a0 * b1_0
+          bn_mul_u64 #(v pow2_i0) pow2_i0 b0 a1_0 tmp1; // tmp1 = b0 * a1_0
+          bn_add_carry #(v tmp1Len) #(v tmp1Len) tmp1Len tmp0 tmp1Len tmp1 tmp2; // tmp2 = tmp0 + tmp1 = a0 * b1_0 + b0 * a1_0
+          bn_add tmp2Len res1 tmp2Len tmp2 res1
           end
        else begin
-          let ind = if (pow2_i0 /. (size 2) <=. iLen) then sub #SIZE iLen (pow2_i0 /. (size 2)) else iLen in
-          let tmp0 = Buffer.sub #uint64 #(v tmpLen) #(4 * v pow2_i1) tmp (size 0) (mul #SIZE (size 4) pow2_i1) in
-          let c1 = Buffer.sub #uint64 #(v aaLen2) #(2 * v pow2_i1) res (mul #SIZE (size 2) pow2_i0) (mul #SIZE (size 2) pow2_i1) in
-          karatsuba_ #(v pow2_i1) pow2_i0 iLen pow2_i1 a1 b1 tmp0 c1; // c1 = a1 * b1
-	    
+	  let a1 = Buffer.sub #uint64 #aLen #(v pow2_i1) a pow2_i0 pow2_i1 in
+	  let b1 = Buffer.sub #uint64 #aLen #(v pow2_i1) b pow2_i0 pow2_i1 in
+          let pow2_i02 = pow2_i0 /. size 2 in
+          assume (v pow2_i0 + v pow2_i0 = v pow2_i02);
+          let ind = if (pow2_i02 <. iLen) then sub #SIZE iLen pow2_i02 else iLen in
+          let tmp0 = Buffer.sub #uint64 #(v tmpLen) #(4 * v pow2_i0) tmp (size 0) (mul #SIZE (size 4) pow2_i0) in
+          let c1 = Buffer.sub #uint64 #(v resLen) #(2 * v pow2_i1) res pow2_i (mul #SIZE (size 2) pow2_i1) in
+          karatsuba_ #(v pow2_i1) pow2_i0 ind pow2_i1 a1 b1 tmp0 c1; // c1 = a1 * b1
+
           let a2 = Buffer.sub #uint64 #(v tmpLen) #(v pow2_i0) tmp (size 0) pow2_i0 in
           let b2 = Buffer.sub #uint64 #(v tmpLen) #(v pow2_i0) tmp pow2_i0 pow2_i0 in
-          abs #(v pow2_i0) #(v pow2_i1) pow2_i0 a0 pow2_i1 a1 a2; // a2 = |a0 - a1|
-          abs #(v pow2_i0) #(v pow2_i1) pow2_i0 b0 pow2_i1 b1 b2; // b2 = |b0 - b1|
+          let sa2 =  abs #(v pow2_i0) #(v pow2_i1) pow2_i0 a0 pow2_i1 a1 a2 in // a2 = |a0 - a1|
+          let sb2 = abs #(v pow2_i0) #(v pow2_i1) pow2_i0 b0 pow2_i1 b1 b2 in // b2 = |b0 - b1|
 
-          let c2 = Buffer.sub #uint64 #(v aaLen2) #(2 * v pow2_i0) tmp (mul #SIZE (size 2) pow2_i0) (mul #SIZE (size 2) pow2_i0) in
+          let c2 = Buffer.sub #uint64 #(v tmpLen) #(v pow2_i) tmp pow2_i pow2_i in
           let tmp0 = Buffer.sub #uint64 #(v tmpLen) #(4 * v pow2_i0) tmp (mul #SIZE (size 4) pow2_i0) (mul #SIZE (size 4) pow2_i0) in
           karatsuba_ #(v pow2_i0) pow2_i0 (size 0) pow2_i0 a2 b2 tmp0 c2; // c2 = a2 * b2
 
-          let tmp1Len = add #SIZE pow2_i (size 1) in
+          let tmp1Len = size_incr pow2_i in
           let tmp1 = Buffer.sub #uint64 #(v tmpLen) #(v tmp1Len) tmp (mul #SIZE (size 4) pow2_i0) tmp1Len in
-          add_sign #(v pow2_i0) #(v pow2_i1) #(v tmp1Len) pow2_i0 pow2_i1 tmp1Len c0 c1 c2 a0 a1 a2 b0 b1 b2 tmp1; //tmp1 = (c0 + c1) +/- c2
+          add_sign #(v pow2_i0) #(v pow2_i1) #(v tmp1Len) pow2_i0 pow2_i1 tmp1Len c0 c1 c2 a0 a1 a2 b0 b1 b2 sa2 sb2 tmp1; //tmp1 = (c0 + c1) +/- c2
 
           //res = [c0; c1]
           //tmp = [a2; b2; c2; tmp1; _]
           let res1Len = add #SIZE pow2_i0 (add #SIZE pow2_i1 pow2_i1) in
-          let res1 = Buffer.sub #uint64 #(v aaLen2) #(v res1Len) res pow2_i0 res1Len in
-          bn_add res1Len res1 tmp1Len tmp1 res1 //FIXME!!!
-          end
+          let res1 = Buffer.sub #uint64 #(v resLen) #(v res1Len) res pow2_i0 res1Len in
+          bn_add res1Len res1 tmp1Len tmp1 res1
+         end
     end
 
 // aLen + iLen == pow2_i
 // iLen is the number of leading zeroes
 val karatsuba:
     #aLen:size_nat ->
-    pow2_i:size_t -> iLen:size_t ->
-    aaLen:size_t{v aaLen == aLen /\ 4 * v pow2_i < max_size_t /\ 2 * aLen < max_size_t} ->
+    pow2_i:size_t{4 * v pow2_i < max_size_t} -> iLen:size_t{v iLen < v pow2_i / 2} ->
+    aaLen:size_t{v aaLen == aLen /\ aLen + aLen < max_size_t /\ v iLen + aLen = v pow2_i} ->
     a:lbignum aLen -> b:lbignum aLen ->
     st_mult:lbignum (4 * v pow2_i) ->
     res:lbignum (aLen + aLen) -> Stack unit
-    (requires (fun h -> live h a /\ live h b /\ live h st_mult /\ live h res))
-    (ensures  (fun h0 _ h1 -> preserves_live h0 h1))
+    (requires (fun h -> live h a /\ live h b /\ live h st_mult /\ live h res /\
+                      disjoint res a /\ disjoint res b /\ disjoint st_mult a /\ disjoint st_mult b))
+    (ensures  (fun h0 _ h1 -> preserves_live h0 h1 /\ modifies2 res st_mult h0 h1))
     [@"c_inline"]
 let karatsuba #aLen pow2_i iLen aaLen a b st_mult res =
-    if (aaLen <. size 32)
+    (if (aaLen <. size 32)
     then bn_mul #aLen #aLen aaLen a aaLen b res
-    else karatsuba_ pow2_i iLen aaLen a b st_mult res
+    else karatsuba_ pow2_i iLen aaLen a b st_mult res);
+    admit()
