code/experimental/rsa/Hacl.Impl.Shift.fst
@@ -13,10 +13,8 @@ inline_for_extraction
 let bn_tbit = u64 0x8000000000000000
 
 val bn_lshift_:
-    #aLen:size_nat ->
-    aaLen:size_t{v aaLen == aLen} ->
-    a:lbignum aLen ->
-    count:size_t -> nw:size_t ->
+    #aLen:size_nat -> aaLen:size_t{v aaLen == aLen} ->
+    a:lbignum aLen -> count:size_t -> nw:size_t ->
     lb:uint32{0 < uint_v #U32 lb /\ uint_v #U32 lb < 64} ->
     res:lbignum aLen{v count + v nw < aLen} -> Stack unit
     (requires (fun h -> live h a /\ live h res))
@@ -26,20 +24,18 @@ let rec bn_lshift_ #aLen aaLen a count nw lb res =
     if (count >. size 0) then begin
        let i = add #SIZE nw count in
        let tmp = res.(i) in
-       let count = sub #SIZE i (size 1) in
+       let count = size_decr count in
        let t1 = a.(count) in
        let rb = u32 64 -. lb in
        assert (0 < uint_v #U32 rb /\ uint_v #U32 rb < 64);
        res.(i) <- tmp |. (shift_right #U64 t1 rb);
        res.(size_decr i) <- shift_left #U64 t1 lb;
-       bn_lshift_ #aLen aaLen a count nw lb res end
+       bn_lshift_ aaLen a count nw lb res end
 
 // res = a << n
 val bn_lshift:
-    #aLen:size_nat ->
-    aaLen:size_t{v aaLen == aLen} ->
-    a:lbignum aLen ->
-    nCount:size_t{0 < v nCount /\ aLen - (v nCount) / 64 - 1 > 0} ->
+    #aLen:size_nat -> aaLen:size_t{v aaLen == aLen} ->
+    a:lbignum aLen -> nCount:size_t{aLen - (v nCount) / 64 > 0} ->
     res:lbignum aLen -> Stack unit
     (requires (fun h -> live h a /\ live h res))
     (ensures (fun h0 _ h1 -> preserves_live h0 h1 /\ modifies1 res h0 h1))
@@ -48,106 +44,103 @@ let bn_lshift #aLen aaLen a nCount res =
     if (nCount =. size 0) then
        copy aaLen a res
     else begin
+       fill aaLen res (u64 0);
        let nw = nCount /. size 64 in
        let lb = nCount %. size 64 in
        if (lb =. size 0) then begin
-          fill aaLen res (u64 0);
           let aLen' = sub #SIZE aaLen nw in
           let a' = Buffer.sub #uint64 #aLen #(v aLen') a (size 0) aLen' in
           let res' = Buffer.sub #uint64 #aLen #(v aLen') res nw aLen' in
           copy aLen' a' res' end
        else begin
-          let count = sub #SIZE aaLen (sub #SIZE nw (size 1)) in
-          bn_lshift_ #aLen aaLen a count nw (size_to_uint32 lb) res end
+          let lb = size_to_uint32 lb in
+          let count = size_decr (sub #SIZE aaLen nw) in
+          let t1 = a.(count) in
+          let i = add #SIZE nw count in
+          res.(i) <- shift_left #U64 t1 lb;
+          bn_lshift_ #aLen aaLen a count nw lb res end
     end
   
 val bn_lshift1_:
-    #aLen:size_nat ->
-    caLen:size_t{v caLen == aLen} -> a:lbignum aLen ->
-    carry:uint64 -> i:size_t{v i <= aLen} ->
+    #aLen:size_nat -> aaLen:size_t{v aaLen == aLen} ->
+    a:lbignum aLen -> carry:uint64 -> i:size_t{v i <= aLen} ->
     res:lbignum aLen -> Stack unit
     (requires (fun h -> live h a /\ live h res))
     (ensures (fun h0 _ h1 -> preserves_live h0 h1 /\ modifies1 res h0 h1))
     [@"c_inline"]
-let rec bn_lshift1_ #aLen caLen a carry i res =
-    if (i <. caLen) then begin
+let rec bn_lshift1_ #aLen aaLen a carry i res =
+    if (i <. aaLen) then begin
         let tmp = a.(i) in
         res.(i) <- (shift_left #U64 tmp (u32 1)) |. carry;
         let carry = if (eq_u64 (logand #U64 tmp bn_tbit) bn_tbit) then u64 1 else u64 0 in
-        bn_lshift1_ #aLen caLen a carry (size_incr i) res
+        bn_lshift1_ aaLen a carry (size_incr i) res
     end
 
-(* res = a << 1 *)
+// res = a << 1
 val bn_lshift1:
-    #aLen:size_nat ->
-    caLen:size_t{v caLen == aLen} -> a:lbignum aLen ->
-    res:lbignum aLen -> Stack unit
+    #aLen:size_nat -> aaLen:size_t{v aaLen == aLen} ->
+    a:lbignum aLen -> res:lbignum aLen -> Stack unit
     (requires (fun h -> live h a /\ live h res))
     (ensures (fun h0 _ h1 -> preserves_live h0 h1 /\ modifies1 res h0 h1))
     [@"c_inline"]
-let bn_lshift1 #aLen caLen a res = bn_lshift1_ #aLen caLen a (u64 0) (size 0) res
+let bn_lshift1 #aLen aaLen a res = bn_lshift1_ aaLen a (u64 0) (size 0) res
 
 val bn_rshift_:
-    #aLen:size_nat ->
-    caLen:size_t{v caLen == aLen} -> a:lbignum aLen ->
-    i:size_t{v i > 0} -> nw:size_t ->
+    #aLen:size_nat -> aaLen:size_t{v aaLen == aLen} ->
+    a:lbignum aLen -> i:size_t{v i > 0} -> nw:size_t ->
     rb:uint32{0 < uint_v #U32 rb /\ uint_v #U32 rb < 64} -> l:uint64 ->
     res:lbignum aLen{v i + v nw <= aLen} -> Stack unit
     (requires (fun h -> live h a /\ live h res))
     (ensures (fun h0 _ h1 -> preserves_live h0 h1 /\ modifies1 res h0 h1))
-
-#reset-options "--z3rlimit 50 --max_fuel 0"
     [@"c_inline"]
-let rec bn_rshift_ #aLen caLen a i nw rb l res =
-    if (i <. sub #SIZE caLen nw) then begin
+let rec bn_rshift_ #aLen aaLen a i nw rb l res =
+    if (i <. sub #SIZE aaLen nw) then begin
         let tmp = l >>. rb in
         let l = a.(add #SIZE nw i) in
         let lb = u32 64 -. rb in
         assert(0 < uint_v #U32 lb /\ uint_v #U32 lb < 64);
         res.(size_decr i) <- tmp |. (shift_left #U64 l lb);
-        bn_rshift_ #aLen caLen a (size_incr i) nw rb l res end
+        bn_rshift_ aaLen a (size_incr i) nw rb l res end
     else res.(size_decr i) <- shift_right #U64 l rb
 
-(* res = a >> n *)
+// res = a >> n
 val bn_rshift:
-    #aLen:size_nat ->
-    caLen:size_t{v caLen == aLen} -> a:lbignum aLen ->
-    nCount:size_t{v nCount > 0 /\ aLen - v nCount / 64 - 1 > 0} ->
+    #aLen:size_nat -> aaLen:size_t{v aaLen == aLen} ->
+    a:lbignum aLen -> nCount:size_t{aLen - v nCount / 64 > 0} ->
     res:lbignum aLen -> Stack unit
     (requires (fun h -> live h a /\ live h res))
     (ensures (fun h0 _ h1 -> preserves_live h0 h1 /\ modifies1 res h0 h1))
     [@"c_inline"]
-let bn_rshift #aLen caLen a nCount res =
+let bn_rshift #aLen aaLen a nCount res =
     if (nCount =. size 0) then
-      copy caLen a res
+      copy aaLen a res
     else begin
       let nw = nCount /. size 64 in
       let rb = nCount %. size 64 in
       (if rb =. size 0 then begin
-          let a_Len = sub #SIZE caLen nw in
-          let a_ = Buffer.sub #uint64 #aLen #(v a_Len) a nw a_Len in
-          let res_ = Buffer.sub #uint64 #aLen #(v a_Len) res (size 0) a_Len in
-          copy a_Len a_ res_ end
+          let aLen' = sub #SIZE aaLen nw in
+          let a' = Buffer.sub #uint64 #aLen #(v aLen') a nw aLen' in
+          let res' = Buffer.sub #uint64 #aLen #(v aLen') res (size 0) aLen' in
+          copy aLen' a' res' end
       else begin
           let l = a.(nw) in
-          bn_rshift_ #aLen caLen a (size 1) nw (size_to_uint32 rb) l res end)
-      end	  
+          bn_rshift_ aaLen a (size 1) nw (size_to_uint32 rb) l res end)
+      end
 
 // res = a % (pow2 nCount)
 val bn_mod_pow2_n:
     #aLen:size_nat -> #resLen:size_nat ->
-    caLen:size_t{v caLen == aLen} -> a:lbignum aLen ->
-    nCount:size_t ->
-    cresLen:size_t{v cresLen == resLen /\ resLen <= aLen /\ resLen - v nCount / 64 - 1 >= 0} ->
+    aaLen:size_t{v aaLen == aLen} -> a:lbignum aLen -> nCount:size_t ->
+    rresLen:size_t{v rresLen == resLen /\ resLen <= aLen /\ resLen - v nCount / 64 > 0} ->
     res:lbignum resLen -> Stack unit
     (requires (fun h -> live h a /\ live h res /\ disjoint res a))
     (ensures (fun h0 _ h1 -> preserves_live h0 h1 /\ modifies1 res h0 h1))
     [@"c_inline"]
-let bn_mod_pow2_n #aLen #resLen caLen a nCount cresLen res =
+let bn_mod_pow2_n #aLen #resLen aaLen a nCount rresLen res =
     let nw = nCount /. size 64 in
     let nb = nCount %. size 64 in
-    let a_ = Buffer.sub a (size 0) cresLen in
-    copy cresLen a_ res;
+    let a' = Buffer.sub a (size 0) rresLen in
+    copy rresLen a' res;
 
     let start_i:size_t =
         if (nb >. size 0) then begin
@@ -156,7 +149,7 @@ let bn_mod_pow2_n #aLen #resLen caLen a nCount cresLen res =
            size_incr nw end
         else nw in
 
-    if (start_i <. cresLen) then begin
-       let res_Len = sub #SIZE cresLen start_i in
-       let res_ = Buffer.sub #uint64 #resLen #(v res_Len) res start_i res_Len in
-       fill res_Len res_ (u64 0) end
+    if (start_i <. rresLen) then begin
+       let resLen' = sub #SIZE rresLen start_i in
+       let res' = Buffer.sub #uint64 #resLen #(v resLen') res start_i resLen' in
+       fill resLen' res' (u64 0) end
